Initial commit: PXL minimal kernel v1.0 (zero placeholders)

PXLFinalProofs/.Makefile.d
@@ -1,0 +1,18 @@
+coq/PXLv3.vo coq/PXLv3.glob coq/PXLv3.v.beautified coq/PXLv3.required_vo: coq/PXLv3.v 
+coq/PXLv3.vos coq/PXLv3.vok coq/PXLv3.required_vos: coq/PXLv3.v 
+coq/PXLv3_Meta.vo coq/PXLv3_Meta.glob coq/PXLv3_Meta.v.beautified coq/PXLv3_Meta.required_vo: coq/PXLv3_Meta.v 
+coq/PXLv3_Meta.vos coq/PXLv3_Meta.vok coq/PXLv3_Meta.required_vos: coq/PXLv3_Meta.v 
+coq/S5_Kripke.vo coq/S5_Kripke.glob coq/S5_Kripke.v.beautified coq/S5_Kripke.required_vo: coq/S5_Kripke.v 
+coq/S5_Kripke.vos coq/S5_Kripke.vok coq/S5_Kripke.required_vos: coq/S5_Kripke.v 
+coq/PXL_Decidability.vo coq/PXL_Decidability.glob coq/PXL_Decidability.v.beautified coq/PXL_Decidability.required_vo: coq/PXL_Decidability.v coq/PXLv3.vo coq/S5_Kripke.vo
+coq/PXL_Decidability.vos coq/PXL_Decidability.vok coq/PXL_Decidability.required_vos: coq/PXL_Decidability.v coq/PXLv3.vos coq/S5_Kripke.vos
+coq/PXL_Completeness_Truth_WF.vo coq/PXL_Completeness_Truth_WF.glob coq/PXL_Completeness_Truth_WF.v.beautified coq/PXL_Completeness_Truth_WF.required_vo: coq/PXL_Completeness_Truth_WF.v coq/PXLv3.vo coq/S5_Kripke.vo coq/PXL_Decidability.vo
+coq/PXL_Completeness_Truth_WF.vos coq/PXL_Completeness_Truth_WF.vok coq/PXL_Completeness_Truth_WF.required_vos: coq/PXL_Completeness_Truth_WF.v coq/PXLv3.vos coq/S5_Kripke.vos coq/PXL_Decidability.vos
+coq/PXL_Completeness_Interface.vo coq/PXL_Completeness_Interface.glob coq/PXL_Completeness_Interface.v.beautified coq/PXL_Completeness_Interface.required_vo: coq/PXL_Completeness_Interface.v coq/PXLv3.vo
+coq/PXL_Completeness_Interface.vos coq/PXL_Completeness_Interface.vok coq/PXL_Completeness_Interface.required_vos: coq/PXL_Completeness_Interface.v coq/PXLv3.vos
+coq/PXL_Completeness_Instance.vo coq/PXL_Completeness_Instance.glob coq/PXL_Completeness_Instance.v.beautified coq/PXL_Completeness_Instance.required_vo: coq/PXL_Completeness_Instance.v coq/PXLv3.vo coq/PXL_Decidability.vo coq/PXL_Completeness_Interface.vo
+coq/PXL_Completeness_Instance.vos coq/PXL_Completeness_Instance.vok coq/PXL_Completeness_Instance.required_vos: coq/PXL_Completeness_Instance.v coq/PXLv3.vos coq/PXL_Decidability.vos coq/PXL_Completeness_Interface.vos
+coq/PXL_TriuneTheory.vo coq/PXL_TriuneTheory.glob coq/PXL_TriuneTheory.v.beautified coq/PXL_TriuneTheory.required_vo: coq/PXL_TriuneTheory.v coq/PXLv3.vo
+coq/PXL_TriuneTheory.vos coq/PXL_TriuneTheory.vok coq/PXL_TriuneTheory.required_vos: coq/PXL_TriuneTheory.v coq/PXLv3.vos
+coq/PXL_TriuneNecessity.vo coq/PXL_TriuneNecessity.glob coq/PXL_TriuneNecessity.v.beautified coq/PXL_TriuneNecessity.required_vo: coq/PXL_TriuneNecessity.v coq/PXLv3.vo
+coq/PXL_TriuneNecessity.vos coq/PXL_TriuneNecessity.vok coq/PXL_TriuneNecessity.required_vos: coq/PXL_TriuneNecessity.v coq/PXLv3.vos
