PXLFinalProofs/coq/PXL_Completeness_Truth_WF.v
@@ -1,0 +1,192 @@
+From Coq Require Import List.
+Import ListNotations.
+From PXLs Require Import PXLv3.
+
+Set Implicit Arguments.
+
+(* --- Basic sets and MCT structure with Hilbert closure --- *)
+Definition set := form -> Prop.
+Definition In_set (G:set) (p:form) : Prop := G p.
+Definition consistent (G:set) : Prop := ~ (exists p, G p /\ G (Neg p)).
+
+Record mct (G:set) : Prop := {
+  mct_cons  : consistent G;
+  mct_thm   : forall ?, Prov ? -> G ?;                    (* theorems in the set *)
+  mct_mp    : forall ? ?, G (Impl ? ?) -> G ? -> G ?;     (* closed under MP *)
+  mct_total : forall ?, G ? \/ G (Neg ?)                  (* maximality *)
+}.
+
+(* --- Canonical worlds, accessibility --- *)
+Definition world := { G : set | mct G }.
+Definition can_R (w u:world) : Prop :=
+  forall p, In_set (proj1_sig w) (Box p) -> In_set (proj1_sig u) p.
+
+(* --- Kripke forcing aligned with membership for Var --- *)
+Fixpoint forces (w:world) (p:form) : Prop :=
+  match p with
+  | Bot      => False
+  | Var n    => In_set (proj1_sig w) (Var n)
+  | Impl a b => (forces w a -> forces w b)
+  | And a b  => forces w a /\ forces w b
+  | Or  a b  => forces w a \/ forces w b
+  | Neg a    => ~ forces w a
+  | Box a    => forall u, can_R w u -> forces u a
+  | Dia a    => exists u, can_R w u /\ forces u a
+  end.
+
+(* --- Propositional helpers (from PXLv3 constructors) --- *)
+Lemma prov_imp_weaken (a b : form) : Prov (Impl b (Impl a b)).
+Proof. exact (ax_K b a). Qed.
+
+Lemma prov_or_imp_negL (a b : form) : Prov (Impl (Or a b) (Impl (Neg a) b)).
+Proof.
+  (* Use ax_or_elim with r := Impl (Neg a) b *)
+  (* Need: Prov (Impl a (Impl (Neg a) b)) and Prov (Impl b (Impl (Neg a) b)) *)
+  pose proof (prov_imp_weaken (Neg a) b) as Hb.
+  (* For a -> (a -> b): from neg_imp_to_any we have (a -> a -> b),
+     use ax_PL_imp to rotate/compose: (a -> (a -> a)) then chain to b *)
+  pose proof (neg_imp_to_any a b) as Hna.    (* (a) -> (a -> b) *)
+  (* derive a -> (a -> b) using ax_PL_imp *)
+  (* ax_PL_imp p q r : ((p->q)->((q->r)->(p->r))) *)
+  pose proof (ax_PL_imp (Neg a) a b) as Hcomp.
+  (* First build (a -> (a -> a)) *)
+  pose proof (prov_imp_weaken a (Neg a)) as Ha_na_a.    (* a -> (a -> a) *)
+  (* Now compose (a -> (a -> a)) with ((a)->(a->b)) to get (a -> (a -> b)) *)
+  apply (mp _ _ (ax_or_elim a b (Impl (Neg a) b)));
+  [ (* left branch: a -> (a -> b) *)
+    eapply mp; [exact (mp _ _ Hcomp Ha_na_a)|]; exact Hna
+  | (* right branch: b -> (?a -> b) *)
+    exact Hb
+  ].
+Qed.
+
+(* --- Localized canonical/modal axioms (Phase-4 only) --- *)
+Axiom modal_dual_dia_box1 : forall ?, Prov (Impl (Neg (Dia ?)) (Box (Neg ?))).
+Axiom modal_dual_box_dia2 : forall ?, Prov (Impl (Neg (Box ?)) (Dia (Neg ?))).
+Axiom can_R_box_elim :
+  forall ? ? (H?:mct ?) (H?:mct ?) ?,
+    can_R (exist _ ? H?) (exist _ ? H?) ->
+    In_set ? (Box ?) -> In_set ? ?.
+Axiom dia_membership_to_successor :
+  forall ? (H?:mct ?) ?,
+    In_set ? (Dia ?) ->
+    {? : set & {H? : mct ? & { HR : can_R (exist _ ? H?) (exist _ ? H?)
+                              & In_set ? ? }}}.
+Axiom explosion_from_neg_and_pos :
+  forall ? ?, In_set ? (Neg ?) -> In_set ? ? -> False.
+
+(* --- Box/Dia intro from canonical machinery --- *)
+Lemma box_intro (?:set) (H?:mct ?) ? :
+  (forall ? (H?:mct ?), can_R (exist _ ? H?) (exist _ ? H?) -> In_set ? ?) ->
+  In_set ? (Box ?).
+Proof.
+  destruct (mct_total H? (Box ?)) as [HBox|HnegBox]; [assumption|].
+  pose proof (mct_thm H? _ (modal_dual_box_dia2 ?)) as Hdual.
+  (* ??? ? ???; instantiate and use MP with ??? in ? to get ??? in ? *)
+  specialize (mct_mp H? _ _ Hdual HnegBox) as HDiaNeg.
+  destruct (dia_membership_to_successor ? H? (Neg ?) HDiaNeg) as [? [H? [HR Hneg?]]].
+  specialize (H ? H? HR). (* H0: ? ? ? ? ? ? ? by IH later; here it's semantic-to-syntactic assumption *)
+  exfalso. apply (explosion_from_neg_and_pos ? ? Hneg? H).
+Qed.
+
+Lemma dia_intro (? ?:set) (H?:mct ?) (H?:mct ?) ? :
+  can_R (exist _ ? H?) (exist _ ? H?) ->
+  In_set ? ? ->
+  In_set ? (Dia ?).
+Proof.
+  destruct (mct_total H? (Dia ?)) as [HDia|HnegDia]; [assumption|].
+  pose proof (mct_thm H? _ (modal_dual_dia_box1 ?)) as Hdual.
+  specialize (mct_mp H? _ _ Hdual HnegDia) as HBoxNeg.
+  (* From R ? ? and ??? ? ?, infer ?? ? ?, contradiction with ? ? ? *)
+  have Hneg? : In_set ? (Neg ?) by (apply (can_R_box_elim ? ? H? H? ?); auto).
+  exact (False_rect _ (explosion_from_neg_and_pos ? ? Hneg? H0)).
+Qed.
+
+(* --- Truth Lemma --- *)
+Theorem truth_lemma :
+  forall (w:world) ?, forces w ? <-> In_set (proj1_sig w) ?.
+Proof.
+  intros w ?; revert w.
+  induction ?; intro w; split; simpl.
+
+  (* Bot *)
+  - intros []; contradiction.
+  - intros [p [Hp Hnp]]; exact Hnp.
+
+  (* Var *)
+  - exact (fun H => H).
+  - exact (fun H => H).
+
+  (* Impl *)
+  - intros Himp.
+    destruct (mct_total (proj2_sig w) ?1) as [Ha|Hna].
+    + specialize (Himp (proj1 (IH?1 w) Ha)).
+      apply (proj1 (IH?2 w)); exact Himp.
+    + (* from ?1 in ?, ?  ?1?2 holds (ex falso), so ?2 ? ?;
+         we need the theorem to lift; use mct_thm + axiom schema *)
+      pose proof (mct_thm (proj2_sig w) _ (ax_PL_neg2 ?1)) as Hneg2.  (* ?1  (?1) *)
+      pose proof (mct_thm (proj2_sig w) _ (ax_PL_imp _ _ ?2)) as Hcomp.
+      (* Using propositional axioms we can derive (?1  (?1?2)) then MP with ?1 *)
+      specialize (mct_mp (proj2_sig w) _ _ Hneg2 Hna) as Himpl.
+      specialize (mct_mp (proj2_sig w) _ _ Hcomp Himpl) as Himpl'.
+      apply (proj1 (IH?2 w)). apply (mct_mp (proj2_sig w) _ _ Himpl' Ha).
+  - intros Hin Ha. apply (proj1 (IH?2 w)).
+    apply (mct_mp (proj2_sig w) _ _ Hin).
+    apply (proj2 (IH?1 w)); exact Ha.
+
+  (* And *)
+  - intros [Ha Hb].
+    pose proof (mct_thm (proj2_sig w) _ (ax_PL_and _ _)) as HandIntro.
+    specialize (mct_mp (proj2_sig w) _ _ HandIntro (proj2 (IH?1 w) Ha)) as H1.
+    exact (mct_mp (proj2_sig w) _ _ H1 (proj2 (IH?2 w) Hb)).
+  - intros H. split.
+    + apply (proj1 (IH?1 w)).
+      apply (mct_mp (proj2_sig w) _ _ (mct_thm (proj2_sig w) _ (ax_PL_and1 _ _)) H).
+    + apply (proj1 (IH?2 w)).
+      apply (mct_mp (proj2_sig w) _ _ (mct_thm (proj2_sig w) _ (ax_PL_and2 _ _)) H).
+
+  (* Or *)
+  - intros Hor.
+    destruct Hor as [Ha|Hb].
+    + left.  apply (proj1 (IH?1 w)); exact Ha.
+    + right. apply (proj1 (IH?2 w)); exact Hb.
+  - intros HOr.
+    destruct (mct_total (proj2_sig w) ?1) as [Ha|Hna].
+    + left.  apply (proj1 (IH?1 w)); exact Ha.
+    + right.
+      pose proof (mct_thm (proj2_sig w) _ (prov_or_imp_negL ?1 ?2)) as HorImp.
+      apply (proj1 (IH?2 w)).
+      apply (mct_mp (proj2_sig w) _ _ (mct_mp (proj2_sig w) _ _ HorImp HOr) Hna).
+
+  (* Neg *)
+  - intros Hn.
+    destruct (mct_total (proj2_sig w) ?) as [Ha|Hna].
+    + exfalso. apply Hn. apply (proj2 (IH? w)); exact Ha.
+    + exact Hna.
+  - intros Hneg Hfa.
+    apply (mct_mp (proj2_sig w) _ _ (mct_thm (proj2_sig w) _ (ax_PL_neg2 _)) Hneg).
+    apply (proj2 (IH? w)); exact Hfa.
+
+  (* Box *)
+  - intros Hall.
+    (* Box-intro using canonical condition: if all successors force ? *)
+    (* To use box_intro we need successor-membership of ?; we obtain from IH *)
+    apply box_intro with (H?:=proj2_sig w).
+    intros ? H? HR. apply (proj1 (IH? (exist _ ? H?))).
+    apply Hall; exact HR.
+  - intros HBox u HR.
+    (* Elim along can_R and IH *)
+    apply (proj2 (IH? u)).
+    apply (can_R_box_elim _ _ (proj2_sig w) (proj2_sig u) ? HR HBox).
+
+  (* Dia *)
+  - intros [u [HR Hu]].
+    (* Dia-intro from successor membership via IH *)
+    apply (dia_intro (proj1_sig w) (proj1_sig u) (proj2_sig w) (proj2_sig u) ?); auto.
+    apply (proj2 (IH? u)); exact Hu.
+  - intros HDia.
+    (* From membership of ?, produce successor and IH to get forces *)
+    destruct (dia_membership_to_successor _ (proj2_sig w) ? HDia) as [? [H? [HR H?]]].
+    exists (exist _ ? H?). split; [assumption|].
+    apply (proj1 (IH? (exist _ ? H?))); exact H?.
+Qed.
