proof_checking/common/PXL_Shims.v
@@ -1,0 +1,9 @@
+Require Import PXLs.proof_checking.pxl_foundation_proof_v1.coq.PXLv3.
+
+Set Implicit Arguments.
+(* constructors *)
+Notation Var  := Atom.
+Notation And  := Conj.
+Notation Or   := Disj.
+(* types *)
+Notation fDisjm := form.  (* undo accidental rename *)
