test.v
@@ -1,0 +1,3 @@
+Require Import PXLs.proof_checking.pxl_foundation_proof_v1.coq.PXLv3.
+
+Check form.
